\documentclass{article}

\usepackage{amsmath}
\usepackage{amssymb}
\usepackage{framed}

\title{Derivation of Word2Vec Models}
\author{Lifu Huang}
\date{Feb. 2016}
\begin{document}
	\maketitle
	\section{CBOW Model}
	Given a word windows of length $C+1$, assume that the index of the the center word in the window is $w_O$, the context words are $w_1, w_2, .., w_C$.
	\subsection{Loss Function}
	\begin{equation}
		\begin{aligned}
			E &=-\log  p(w_{O}|w_{1}, w_{2}, .., w_{C})\\ 
			&=-\log  \left( \frac { e^{ u_{w_{O}} } }{ \sum _{ k=1 }^{ V } e^{ u_{ k } } }  \right) \\ 
			&=-u_{w_{O}}+\log { \sum _{ k=1 }^{ V } e^{ u_{ k } } } 
		\end{aligned}
	\end{equation}
	\subsection{Updating W'}
	\begin{equation}
		\begin{aligned}
			\delta'_i &= \frac{\partial E}{\partial u_{i}} \\
			&= -t_i + \frac{e^{u_i}}{\sum_{k=1}^{V}e^{u_{k}}} \\
			&= y_i - t_i \\
		\end{aligned}
	\end{equation}

	\begin{equation}
		\begin{aligned}
			\delta' = \nabla_u E = y - t \\		
		\end{aligned}
	\end{equation}
	
	\begin{equation}
		\begin{aligned}
			\frac{\partial E}{\partial W'_{ij}} &= \sum_{k=1}^{V} \left( \frac{\partial E}{\partial u_k} \cdot \frac{\partial u_k}{\partial W'_{ij}} \right) \\
			&= \sum_{k=1}^{V} \left(\delta'_k \cdot \frac{\partial u_k}{\partial W'_{ij}}\right)  \\
			&= \delta'_k \cdot h_j \\
		\end{aligned}
	\end{equation}	

	\begin{equation}
		\begin{aligned}	
			\nabla_{W'} E &= \delta' \cdot h^T
		\end{aligned}
	\end{equation}
	
	\subsubsection*{Updating Rules}
	\begin{framed}
	\begin{equation}
		\begin{aligned}
			v'_{i, new} &= v'_{i, old} - \eta \cdot \delta'_i \cdot h &\mbox{for i = 1, 2, .., V}\\
		\end{aligned}
	\end{equation}
	\end{framed}
	
	\subsection{Updating W}
	\begin{equation}
		\begin{aligned}
			\delta_i &= \frac{\partial E}{\partial h_i} \\
			&= \sum_{j=1}^{V} \frac{\partial E}{\partial u_j} \cdot \frac{\partial u_j}{\partial h_i} \\
			&= \sum_{j=1}^{V} \delta'_j \cdot W'_{ji} 
		\end{aligned}
	\end{equation}
	
	\begin{equation}
		\begin{aligned}
			\delta &= (W')^T \cdot \delta'
		\end{aligned}
	\end{equation}
	
	\begin{equation}
		\begin{aligned}
			\frac{\partial E}{W_{ij}} &= \sum_{k=1}^{N} \frac{\partial E}{h_k} \cdot \frac{\partial h_k}{\partial W_{ij}} \\
			&= \sum_{k=1}^{N} \delta_k \cdot \frac{\partial}{\partial W_{ij}} \left(\frac{1}{C} \sum_{c=1}^{C} W_{k\cdot} \cdot x_{w_{c}} \right)\\
			&= \frac{1}{C} \cdot \delta_i \cdot \sum_{c=1}^{C} x_{w_{c}, j}
		\end{aligned}
	\end{equation}
	
	\begin{equation}
		\begin{aligned}
			\nabla_W E &= \frac{1}{C} \cdot \delta \cdot \left(\sum_{c=1}^{C} x_{w_{c}}\right)^T \\
		\end{aligned}
	\end{equation}
	
	\subsubsection*{Updating Rules}
	\begin{framed}
	\begin{equation}
		\begin{aligned}
			v_{w_i, new} &= v_{w_i, old} - \eta \cdot \frac{1}{C} \cdot \delta &\mbox{for i = 1, 2, .., C}
		\end{aligned}
	\end{equation}
	\end{framed}
	
	\newpage
	\section{Skip-Gram Model}
	Given a word windows of length $C+1$, assume that the index of the the center word in the window is $w_I$, the context words are $w_1, w_2, .., w_C$.
	\subsection{Loss Function}
	\begin{equation}
		\begin{aligned}
			E &=-\log p(w_{1}, w_{2}, .., w_{C}|w_{I})\\ 
			&= -\log \prod_{c=1}^{C} p(w_{c}|w_{I}) \\
			&= -\sum_{c=1}^{C} \log p(w_{c}|w_{I}) \\ 
			&= -\sum_{c=1}^{C} \log \frac{e^{u_{c,w_c}}}{\sum_{k=1}^{V}e^{u_{ck}}} \\ 
		\end{aligned}
	\end{equation}
	
	\subsection{Updating W'}
	\begin{equation}
		\begin{aligned}
			\delta'_{ci} &= \frac{\partial E}{\partial u_{ci}} \\
			&= \frac{\partial}{\partial u_{ci}} \left(
			-\sum_{c=1}^{C} \log \frac{e^{u_{c,w_c}}}{\sum_{k=1}^{V}e^{u_{ck}}} \right) \\
			&= -t_{ci} + \frac{e^{u_{ci}}}{\sum_{k=1}^{V}e^{u_{ck}}} \\
			&= y_{ci} - t_{ci}
		\end{aligned}
	\end{equation}
	
	\begin{equation}
		\begin{aligned}
			\delta'_{c} &= y_{c} - t_{c} 
		\end{aligned}
	\end{equation}

	\begin{equation}
		\begin{aligned}
			\frac{\partial E}{\partial W'_{ij}} &= \sum_{c=1}^{C} \sum_{k=1}^{V} \frac{\partial E}{\partial u_{ck}} \cdot \frac{\partial u_{ck}}{\partial W'_{ij}} \\
			&= \sum_{c=1}^{C} \sum_{k=1}^{V} \delta'_{ck} \cdot \frac{\partial}{\partial W'_{ij}}\sum_{l=1}^{N} W'_{kl} \cdot h_l \\
			&= \left(\sum_{c=1}^{C} \delta'_{ci} \right)\cdot h_j \\
			&= \gamma_i \cdot h_j
		\end{aligned}	
	\end{equation}
	
	\begin{equation}
		\begin{aligned}
			\nabla_{W'} E &= \gamma \cdot h^T
		\end{aligned}	
	\end{equation}
	
	\subsubsection*{Updating Rules}
	\begin{framed}
	\begin{equation}
		\begin{aligned}
			v'_{i, new} &= v'_{i, old} - \eta \cdot \gamma_i \cdot h &\mbox{for i = 1, 2, .., V}
		\end{aligned}
	\end{equation}
	\end{framed}
	
	\subsection{Updating W}
	\begin{equation}
		\begin{aligned}
			\delta_i &= \frac{\partial E}{\partial h_i} \\
			&= \sum_{c=1}^{C}\sum_{j=1}^{V} \left( \frac{\partial E}{u_{cj}} \cdot \frac{\partial u_{cj}}{\partial h_i}\right)  \\
			&= \sum_{c=1}^{C}\sum_{j=1}^{V}\left( \delta'_{cj}\cdot W'_{j,i} \right)   \\
			&= \sum_{j=1}^{V} W'_{ji} \cdot \left(\sum_{c=1}^{C} \delta'_{cj} \right) \\
			&= \sum_{j=1}^{V} W'_{ji} \cdot \gamma_j
		\end{aligned}
	\end{equation}
	
	\begin{equation}
		\begin{aligned}
			\delta = (W')^T \cdot \gamma
		\end{aligned}
	\end{equation}
	
	\begin{equation}
		\begin{aligned}
			\frac{\partial E}{\partial W_{ij}} &= \sum_{k=1}^{N} \left( \frac{\partial E}{\partial h_k} \cdot \frac{\partial h_k}{\partial W_{ij}}\right) \\
			&= \sum_{k=1}^{N} \left( \delta_k \cdot \frac{\partial h_k}{W_{ij}}\right) \\
			&= \delta_i \cdot x_{w_I,j} \\
		\end{aligned}
	\end{equation}
	
	
	\begin{equation}
		\begin{aligned}
			\nabla_W E = \delta \cdot x_{w_I}^T
		\end{aligned}
	\end{equation}
	
	\subsubsection*{Updating Rules}
	\begin{framed}
	\begin{equation}
		\begin{aligned}
			v_{w_I, new} &= v_{w_I, old} - \eta \cdot \delta
		\end{aligned}
	\end{equation}
	\end{framed}
	
	\newpage
	\section{Negative Sampling}
	
The derivation for negative sampling is almost the same as before, except that we changed our objective function to its  approximated version for better performance. As a result, all we need is to recalculate $\delta'$, which can then be plugged back into formula in CBOW or Skip-Gram model we derived before.
	\subsection {CBOW} 
	\begin{equation}
		\begin{aligned}
			E &= -\log \sigma(u_{w_O}) - \sum_{k \sim P_n(w)} \log \sigma (-u_{k}) 
		\end{aligned}
	\end{equation}
	\begin{equation}
		\begin{aligned}
			\delta'_{i} &= \frac{\partial E}{\partial u_{i}} \\
			&= 
			\begin{cases}
				\sigma(u_{i}) - t_{i} &\mbox{for $i \in \{w_O\} \cup \{k \sim P_n(w) \}$}\\
				0  &\mbox{Otherwise}
			\end{cases}
		\end{aligned}
	\end{equation}
	
	\subsubsection*{Complete Updating Rules}

	\begin{framed}
	\centering
	Let $S = \{w_O\} \cup \{k \sim P_n(w) \}$,
	\begin{equation}
		\begin{aligned}
			\delta'_{i} &= \frac{\partial E}{\partial u_{i}} = \sigma(u_{i}) - t_{i} &\mbox{for $i \in S$}
		\end{aligned}
	\end{equation}
		
	\begin{equation}
		\begin{aligned}
			v'_{i, new} &= v'_{i, old} - \eta \cdot \delta'_i \cdot h  &\mbox{for $i \in S$}\\
		\end{aligned}
	\end{equation}
	
	\begin{equation}
		\begin{aligned}
		\delta &= \sum_{i \in S} \delta'_{i} \cdot v'_{i}
		\end{aligned}
	\end{equation}
	
	\begin{equation}
		\begin{aligned}
			v_{w_i, new} &= v_{w_i, old} - \eta \cdot \frac{1}{C} \cdot \delta &\mbox{for i = 1, 2, .., C}
		\end{aligned}
	\end{equation}
			
	\end{framed}
	
	\subsection {Skip-Gram} 

	\begin{equation}
		\begin{aligned}
			E &= \sum_{c=1}^{C} \left( -\log \sigma(u_{c,w_c}) -  \sum_{k \sim P_n(w)} \log \sigma (-u_{c,k})  \right)
		\end{aligned}
	\end{equation}
	
	\begin{equation}
		\begin{aligned}
			\delta'_{ci} &= \frac{\partial E}{\partial u_{ci}} \\
			&=
			\begin{cases}
				\sigma(u_{ci}) - t_{ci}  &\mbox{for $i \in \{w_c\} \cup \{k \sim P_n(w) \}$}\\
				0  &\mbox{Otherwise}
			\end{cases}
		\end{aligned}
	\end{equation}
	
	\subsubsection*{Complete Updating Rules}
	For each context word $w_c$, 
	\begin{framed}
	\centering
	let $S_{c} = \{w_c\} \cup \{k \sim P_n(w) \}$, \\
	\begin{equation}
	\begin{aligned}
		\delta'_{ci} &= \frac{\partial E}{\partial u_{ci}} = \sigma(u_{ci}) - t_{ci} &\mbox{for $i \in S_c$}
	\end{aligned}
	\end{equation}
	
	\begin{equation}
	\begin{aligned}
		v'_{i, new} &= v'_{i, old} - \eta \cdot \delta'_{ci} \cdot h  &\mbox{for $i \in S_c$}\\
	\end{aligned}
	\end{equation}
	
	\begin{equation}
	\begin{aligned}
		\delta_c &= \sum_{i \in S_c} \delta'_{ci} \cdot v'_{i}
	\end{aligned}
	\end{equation}
	
	\begin{equation}
	\begin{aligned}
		v_{w_I, new} &= v_{w_I, old} - \eta \cdot \delta_c 
	\end{aligned}
	\end{equation}
	\end{framed}
\end{document}