\documentclass{article}

\usepackage{amsmath}
\usepackage{amssymb}

\title{Derivation of (Deep) RNN}
\author{Lifu Huang}
\date{Mar. 2016}
\begin{document}
	\maketitle
	\section{Loss Function}
	\begin{equation}
	\begin{aligned}
		J &= \frac{1}{T}\sum_{t=1}^{T} J^{(t)} \\
		&= \frac{1}{T}\sum_{t=1}^{T} \sum_{j=1}^{|V|} -y^{(t)}_j \log \hat{y}^{(t)}_j \\
		&= \frac{1}{T} \sum_{t=1}^T -\log{\hat{y}_k^{(t)}}	
	\end{aligned}
	\end{equation}
	
	\begin{equation}
	\begin{aligned}	
		J^{(t)} &= -\log{\hat{y}^{(t)}_k}
	\end{aligned}
	\end{equation}
	
	\section{Forward Propagation}
	Assume that we have a $n+1$ layer Recurrent Neural Network,
	\begin{equation}
	\begin{aligned}
		\hat{y}^{(t)} &= g(z^{(n)(t)}) 
	\end{aligned}	
	\end{equation}
	
	\begin{equation}
	\begin{aligned}
		h^{(l)(t)} &= 
		\begin{cases}
			f(z^{(l-1)(t)}) &0 < l < n\\
			x^{(t)} &l = 0
		\end{cases}	
	\end{aligned}	
	\end{equation}
	
	\begin{equation}
	\begin{aligned}
		z^{(l)(t)} &= 
		\begin{cases}
			W^{(l)} h^{(l-1)(t)} + b^{(l)} &l = n\\
			H^{(l)} h^{(l)(t-1)} + W^{(l)} h^{(l-1)(t)} + b^{(l)} &0 < l < n
		\end{cases}
	\end{aligned}
	\end{equation}
	\newpage
	\section{Backward Propagation}
	For the purpose of simplicity, all derivation in this chapter will be made with respect to the loss function of a single time step. Moreover, we will presume that $g(x)$ here is the softmax function, which can be easily substituted with any other functions as needed. 
	\subsection{Derivation of $\delta$s}
	\subsubsection{The Output Layer}
	\begin{equation}
	\begin{aligned}
		\frac{\partial J^{(t)}}{\partial z^{(n)(t)}} 
		&= \frac{\partial}{\partial z^{(n)(t)}} (-\log{\hat{y}^{(t)}_k}) \\
		&= \frac{\partial}{\partial z^{(n)(t)}} (-z^{(n)(t)}_k + \log{\sum_{j=1}^{|V|} z^{(n)(t)}_j}) \\
		&= (\hat{y}^{(t)} - y^{(t)})^T 
	\end{aligned}
	\end{equation}
	
	\begin{equation}
	\begin{aligned}
		\delta^{(n)(t)} 
		&= \nabla_{z^{(n)(t)}} J^{(t)} \\
		&= \hat{y}^{(t)} - y^{(t)} 
	\end{aligned}
	\end{equation}
	
	\subsubsection{Top Hidden Layer}
	\begin{equation}
		\begin{aligned}
		\frac{\partial J^{(t)}}{\partial z^{(n-1)(t)}} 
		&= \frac{\partial J^{(t)}}{\partial z^{(n)(t)}} 
		\frac{\partial z^{(n)(t)}}{\partial z^{(n-1)(t)}} \\
		&= (\delta^{(n)(t)})^T  \frac{\partial}{\partial z^{(n-1)(t)}} (W^{(n)} f(z^{(n-1)(t)}) + b^{(n)})\\
		&= (\delta^{(n)(t)})^T  W^{(n)}  diag[f'(z^{(n-1)(t)})]
		\end{aligned}
	\end{equation}
	
	\begin{equation}
	\begin{aligned}
		\delta^{(n-1)(t)} 
		&= \nabla_{z^{(n-1)(t)}} J^{(t)} \\
		&= diag[f'(z^{(n-1)(t)})] (W^{(n)})^T \delta^{(n)(t)}
	\end{aligned}
	\end{equation}
	
	\begin{equation}
	\begin{aligned}
		\frac{\partial J^{(t)}}{\partial z^{(n-1)(t-c)}} 
		&= \frac{\partial J^{(t)}}{\partial z^{(n-1)(t-c+1)}} 
		\frac{\partial z^{(n-1)(t-c+1)}}{\partial z^{(n-1)(t-c)}} \\
		&= (\delta^{(n-1)(t-c+1)})^T \frac{\partial}{\partial z^{(n-1)(t-c)}} (H^{(n-1)} h^{(n-1)(t-c)} + W^{(n-1)} h^{(n-2)(t-c+1)} + b^{(n-1)})\\		
		&= (\delta^{(n-1)(t-c+1)})^T \frac{\partial}{\partial z^{(n-1)(t-c)}} (H^{(n-1)} f(z^{(n-1)(t-c)}))\\
		&= (\delta^{(n-1)(t-c+1)})^T H^{(n-1)} diag[f'(z^{(n-1)(t-c)})]
	\end{aligned}
	\end{equation}
		
	\begin{equation}
	\begin{aligned}
		\delta^{(n-1)(t-c)} 
		&= \nabla_{z^{(n-1)(t-c)}} J^{(t)} \\
		&= diag[f'(z^{(n-1)(t-c)})] (H^{(n-1)})^T \delta^{(n-1)(t-c+1)}
	\end{aligned}
	\end{equation}
	
	\subsubsection{Other Hidden Layers}
	\begin{equation}
	\begin{aligned}
		\frac{\partial J^{(t)}}{\partial z^{(l)(t)}} 
		&= \frac{\partial J^{(t)}}{\partial z^{(l+1)(t)}} 
		\frac{\partial z^{(l+1)(t)}}{\partial z^{(l)(t)}} \\
		&= (\delta^{(l+1)(t)})^T \frac{\partial}{\partial z^{(l)(t)}} (H^{(l+1)} h^{(l+1)(t-1)} + W^{(l+1)} h^{(l)(t)} + b^{(l+1)})\\
		&= (\delta^{(l+1)(t)})^T \frac{\partial}{\partial z^{(l)(t)}} (W^{(l+1)} f(z^{(l)(t)}))\\
		&= (\delta^{(l+1)(t)})^T W^{(l+1)} diag[f'(z^{(l)(t)})]
	\end{aligned}
	\end{equation}
		
	\begin{equation}
	\begin{aligned}
		\delta^{(l)(t)} 
		&= \nabla_{z^{(l)(t)}} J^{(t)} \\
		&= diag[f'(z^{(l)(t)})] (W^{(l+1)})^T \delta^{(l+1)(t)}
	\end{aligned}
	\end{equation}
	
	\begin{equation}
	\begin{aligned}
		\frac{\partial J^{(t)}}{\partial z^{(l)(t-c)}} 
		&= \left(\frac{\partial J^{(t)}}{\partial z^{(l)(t-c+1)}} 
		\frac{\partial z^{(l)(t-c+1)}}{\partial z^{(l)(t-c)}}\right) + \left(\frac{\partial J^{(t)}}{\partial z^{(l+1)(t-c)}} 
		\frac{\partial z^{(l+1)(t-c)}}{\partial z^{(l)(t-c)}}\right)\\
		&= \left((\delta^{(l)(t-c+1)})^T \frac{\partial}{\partial z^{(l)(t-c)}} (H^{(l)} h^{(l)(t-c)} + W^{(l)} h^{(l-1)(t-c+1)} + b^{(l)}) \right) +\\
		& \left( (\delta^{(l+1)(t-c)})^T \frac{\partial}{\partial z^{(l)(t-c)}}(H^{(l+1)} h^{(l+1)(t-c-1)} + W^{(l+1)} h^{(l)(t-c)} + b^{(l+1)}) \right)\\
		&= \left((\delta^{(l)(t-c+1)})^T \frac{\partial}{\partial z^{(l)(t-c)}} (H^{(l)} f(z^{(l)(t-c)}))\right) +\\
		&\left( (\delta^{(l+1)(t-c)})^T \frac{\partial}{\partial z^{(l)(t-c)}}(W^{(l+1)} f(z^{(l)(t-c)}))\right)\\
		&= (\delta^{(l)(t-c+1)})^T H^{(l)} diag[f'(z^{(l)(t-c)})] + 
		(\delta^{(l+1)(t-c)})^T W^{(l+1)} diag[f'(z^{(l)(t-c)})] \\
		&= ((\delta^{(l)(t-c+1)})^T H^{(l)} + 
		(\delta^{(l+1)(t-c)})^T W^{(l+1)}) diag[f'(z^{(l)(t-c)})]  
	\end{aligned}
	\end{equation}
	
	\begin{equation}
	\begin{aligned}
		\delta^{(l)(t-c)} &= \nabla_{z^{(l)(t-c)}} J^{(t)} \\
		&= diag[f'(z^{(l)(t-c)})] ((H^{(l)})^T \delta^{(l)(t-c+1)} + W^{(l+1)} (\delta^{(l+1)(t-c)})^T)
	\end{aligned}
	\end{equation}
	
	\subsection{Gradients of Parameters}
	
	\paragraph{$H$ -- horizontally propagation matrix}
	\begin{equation}
	\begin{aligned}
		\frac{\partial J^{(t)}}{\partial H^{(l)}} 
		&= \sum_{k=1}^{t} \frac{\partial J^{(t)}}{\partial H^{(l)}}\bigg|_{(k)}  \\
		&= \sum_{k=1}^{t}
		\frac{\partial J^{(t)}}{\partial z^{(l)(k)}} 
		\frac {\partial z^{(l)(k)}}{\partial H^{(l)}}\bigg|_{(k)} \\
		&= \sum_{k=1}^{t}
		(\delta^{(l)(k)})^T \left[\frac{\partial }{\partial H^{(l)}} (\epsilon_i)^T (H^{(l)} h^{(l)(k-1)} +  W^{(l)} h^{(l-1)(k)} + b^{(l)})\right] \\
		&= \sum_{k=1}^{t}
		(\delta^{(l)(k)})^T \left[h^{(l)(k-1)} (\epsilon_i)^T\right]\\	
		&= \sum_{k=1}^{t} h^{(l)(k-1)} (\delta^{(l)(k)})^T
	\end{aligned}
	\end{equation}
	
	\begin{equation}
	\begin{aligned}
		\nabla_{H^{(l)}} J^{(t)} &= \sum_{k=1}^{t} \delta^{(1)(k)}  (h^{(l)(k-1)})^T
	\end{aligned}
	\end{equation}
	
	\paragraph{$W$ -- vertically propagation matrix}
	\begin{equation}
	\begin{aligned}
	\frac{\partial J^{(t)}}{\partial W^{(n)}} 
	&= \frac{\partial J^{(t)}}{\partial z^{(n)(t)}} 
	\frac{\partial z^{(n)(t)}}{\partial W^{(n)}} \\
	&= (\delta^{(n)(t)})^T \left[\frac{\partial z^{(n)(t)}_i}{\partial W^{(n)}}\right]\\
	&= (\delta^{(n)(t)})^T \left[\frac{\partial }{\partial W^{(n)}} ((\epsilon_i)^T  W^{(n)} h^{(n-1)(t)} + b^{(n)}_i)\right]\\
	&= (\delta^{(n)(t)})^T \left[h^{(n-1)(t)} (\epsilon_i)^T\right]\\	
	&= h^{(n-1)(t)} (\delta^{(n)(t)})^T
	\end{aligned}
	\end{equation}
	
	\begin{equation}
	\begin{aligned}
	\nabla_{W^{(n)}} J^{(t)} &= \delta^{(n)(t)} (h^{(n-1)(t)})^T\\
	\end{aligned}
	\end{equation}
	
	\begin{equation}
	\begin{aligned}
		\frac{\partial J^{(t)}}{\partial W^{(l)}} &= \sum_{k=1}^{t} \frac{\partial J^{(t)}}{\partial W^{(l)}}\bigg|_{(k)}  \\
		&= \sum_{k=1}^{t}
		\frac{\partial J^{(t)}}{\partial z^{(l)(k)}} 
		\frac{\partial z^{(l)(k)}}{\partial W^{(l)}}\bigg|_{(k)} \\
		&= \sum_{k=1}^{t}
		(\delta^{(l)(k)})^T \left[\frac{\partial }{\partial W^{(l)}}(\epsilon_i)^T (H^{(l)} h^{(l)(k-1)} + W^{(l)} h^{(l-1)(k)} + b^{(l)})\right] \\
		&= \sum_{k=1}^{t}
		(\delta^{(l)(k)})^T \left[h^{(l-1)(k)} (\epsilon_i)^T\right]\\	
		&= \sum_{k=1}^{t} h^{(l-1)(k)} (\delta^{(l)(k)})^T
	\end{aligned}
	\end{equation}
	
	\begin{equation}
	\begin{aligned}
		\nabla_{W^{(l)}} J^{(t)} &= \sum_{k=1}^{t} \delta^{(l)(k)}  (h^{(l-1)(k)})^T
	\end{aligned}
	\end{equation}	
		
	\paragraph{b -- bias term}
	\begin{equation}
	\begin{aligned}
	\frac{\partial J^{(t)}}{\partial b^{(n)}} &= \frac{\partial J^{(t)}}{\partial z^{(n)(t)}} 
	\frac{\partial z^{(n)(t)}}{\partial b^{(n)}} \\
	&= (\delta^{(n)(t)})^T I \\
	&= (\delta^{(n)(t)})^T 
	\end{aligned}
	\end{equation}
	
	\begin{equation}
	\begin{aligned}
	\nabla_{b^{(n)}} J^{(t)} &= \delta^{(n)(t)} 
	\end{aligned}
	\end{equation}
	
	\begin{equation}
	\begin{aligned}
		\frac{\partial J^{(t)}}{\partial b^{(l)}} &= \sum_{k=1}^{t} \frac{\partial J^{(t)}}{\partial b^{(l)}}\bigg|_{(k)}  \\
		&= \sum_{k=1}^{t}
		\frac{\partial J^{(t)}}{\partial z^{(l)(k)}} 
		\frac{\partial z^{(l)(k)}}{\partial b^{(l)}}\bigg|_{(k)} \\
		&= \sum_{k=1}^{t}
		(\delta^{(l)(k)})^T I \\
		&= \sum_{k=1}^{t} (\delta^{(l)(k)})^T
	\end{aligned}
	\end{equation}
	
	\begin{equation}
	\begin{aligned}
		\nabla_{b^{(l)}} J^{(t)} &= \sum_{k=1}^{t} \delta^{(l)(k)} \\
	\end{aligned}
	\end{equation}	
	
	\subsection{Conclusion}
	\begin{align}
		\delta^{(n)(t)} &= \hat{y}^{(t)} - y^{(t)} \\
		\delta^{(n-1)(t)} &= diag[f'(z^{(n-1)(t)})] (W^{(n)})^T \delta^{(n)(t)} \\
		\delta^{(n-1)(t-c)} &= diag[f'(z^{(n-1)(t-c)})] (H^{(n-1)})^T \delta^{(n-1)(t-c+1)} \\
		\delta^{(l)(t)} &= diag[f'(z^{(l)(t)})] (W^{(l+1)})^T \delta^{(l+1)(t)} \\
		\delta^{(l)(t-c)} &= diag[f'(z^{(l)(t-c)})] ((H^{(l)})^T \delta^{(l)(t-c+1)} + (W^{(l+1)})^T \delta^{(l+1)(t-c)}) \\
		\nabla_{H^{(l)}} J^{(t)} &= \sum_{k=1}^{t} \delta^{(l)(t)} (h^{(l)(k-1)})^T \\
		\nabla_{W^{(n)}} J^{(t)} &= \delta^{(n)(t)} (h^{(n-1)(t)})^T \\
		\nabla_{W^{(l)}} J^{(t)} &= \sum_{k=1}^{t} \delta^{(l)(k)} (h^{(l-1)(k)})^T \\
		\nabla_{b^{(n)}} J^{(t)} &= \delta^{(n)(t)} \\
		\nabla_{b^{(l)}} J^{(t)} &= \sum_{k=1}^{t} \delta^{(l)(k)}
	\end{align}
	
	\newpage
	\section{Trick for Implementation}
	Derivation above is made with respect to the loss function of a single time step, (i.e. $\nabla J^{(t)}$). When taking derivative of the final loss function $\nabla J$ with respect to $H^{(l)}$, $W^{(l)}$, and $b^{(l)}$ for $l < n$, instead of calculate $\nabla J^{(t)}$ for every time step and sum them up at last, which is correct but inefficient, we backprop only once by keeping record of $\gamma^{(l)(t)}$, which is the accumulating sum of $\delta^{(l)(t)(i)}$ over range $t$ to $T$.\footnote{We will slightly change our notation here by adding one more superscript to $\delta$ so as to differentiate $\delta$ from different $J^{(t)}$, now $\delta^{(l)(t)(i)} = \nabla_{z^{(l)(t)}}J^{(i)}$.} \\\\
	It is easy to find that, when $t = T-1$:\\
	\begin{equation}
	\begin{aligned}
		\gamma^{(l)(t)} &= \delta^{(l)(t)(t)} \\
	\end{aligned}
	\end{equation}
	
	when $1 \le t \le T-1$:
	\begin{equation}
	\begin{aligned}
		\gamma^{(n-1)(t)} 
		&= \sum_{i=t}^{T} \delta^{(n-1)(t)(i)} \\
		&= \delta^{(n-1)(t)(t)} + \sum_{i=t+1}^{T} \delta^{(n-1)(t)(i)} \\
		&= \delta^{(n-1)(t)(t)} + \sum_{i=t+1}^{T} diag[f'(z^{(n-1)(t)})] (H^{(n-1)})^T \delta^{(n-1)(t+1)(i)}\\
		&= \delta^{(n-1)(t)(t)} + diag[f'(z^{(n-1)(t)})] (H^{(n-1)})^T \sum_{i=t+1}^{T} \delta^{(n-1)(t+1)(i)}\\
		&= \delta^{(n-1)(t)(t)} + diag[f'(z^{(n-1)(t)})] (H^{(n-1)})^T \gamma^{(n-1)(t+1)} \\
		&= \delta^{(n-1)(t)(t)} + f'(z^{(n-1)(t)})\circ ((H^{(n-1)})^T \gamma^{(n-1)(t+1)})
	\end{aligned}
	\end{equation}
	
	when $1 \le t \le T-1$ and $1 \le l \le n-2$:
	\begin{equation}
	\begin{aligned}
		\gamma^{(l)(t)} 
		&= \sum_{i=t}^{T} \delta^{(l)(t)(i)} \\
		&= \sum_{i=t}^{T} diag[f'(z^{(l)(t)})] ((H^{(l)})^T \delta^{(l)(t+1)(i)} + (W^{(l+1)})^T \delta^{(l+1)(t)(i)}) \\
		&= \delta^{(l)(t)(t)} + \sum_{i=t+1}^{T} \delta^{(l)(t)(i)} \\
		&= \delta^{(l)(t)(t)} + \sum_{i=t+1}^{T} diag[f'(z^{(l)(t)})] ((H^{(l)})^T \delta^{(l)(t+1)(i)} + (W^{(l+1)})^T \delta^{(l+1)(t)(i)}) \\
		&= \delta^{(l)(t)(t)} + diag[f'(z^{(l)(t)})] \\
		&\left( (H^{(l)})^T \left(\sum_{i=t+1}^{T} \delta^{(l)(t+1)(i)}\right) + (W^{(l+1)})^T \left(\sum_{i=t+1}^{T} \delta^{(l+1)(t)(i)}\right) \right) \\		
		&= \delta^{(l)(t)(t)} + f'(z^{(l)(t)}) \circ ( (H^{(l)})^T \gamma^{(l)(t+1)} + (W^{(l+1)})^T (\gamma^{(l+1)(t)} - \delta^{(l+1)(t)(t)})) \\
		&= f'(z^{(l)(t)}) \circ ( (H^{(l)})^T \gamma^{(l)(t+1)} + (W^{(l+1)})^T \gamma^{(l+1)(t)})
	\end{aligned}
	\end{equation}
	
	We can now simplify our gradients by reorganizing terms and using $\gamma$s instead of $\delta$s,
	\begin{equation}
	\begin{aligned}
		\nabla_{H^{(l)}} J 
		&= \frac{1}{T}\sum_{i=1}^{T} \sum_{j=1}^{i} \delta^{(l)(j)(i)}  (h^{(j-1)})^T\\
		&= \frac{1}{T} \sum_{i=1}^{T} \sum_{j=i}^{T} \delta^{(l)(i)(j)}  (h^{(l)(i-1)})^T\\
		&= \frac{1}{T} \sum_{i=1}^{T} \gamma^{(l)(i)}  (h^{(l)(i-1)})^T\\
	\end{aligned}
	\end{equation}
	
	\begin{equation}
	\begin{aligned}
		\nabla_{W^{(l)}} J 
		&= \frac{1}{T} \sum_{i=1}^{T} \sum_{j=1}^{i} \delta^{(l)(j)(i)}  (h^{(l-1)(j)})^T\\
		&= \frac{1}{T} \sum_{i=1}^{T} \sum_{j=i}^{T} \delta^{(l)(i)(j)}  (h^{(l-1)(i)})^T\\
		&= \frac{1}{T} \sum_{i=1}^{T} \gamma^{(l)(i)}  (h^{(l-1)(i)})^T\\
	\end{aligned}
	\end{equation}
	
	\begin{equation}
	\begin{aligned}
		\nabla_{b^{(l)}} J 
		&= \frac{1}{T} \sum_{i=1}^{T} \sum_{j=1}^{i} \delta^{(l)(j)(i)} \\
		&= \frac{1}{T} \sum_{i=1}^{T} \sum_{j=i}^{T} \delta^{(l)(i)(j)} \\
		&= \frac{1}{T} \sum_{i=1}^{T} \gamma^{(l)(i)} \\
	\end{aligned}
	\end{equation}
	Hmm, now we can put every thing together,
	\begin{align}
		\delta^{(l)(t)(t)} &=
		\begin{cases}
			\hat{y}^{(t)} - y^{(t)} &l=n\\	
			f'(z^{(l)(t)}) \circ ((W^{(l+1)})^T \delta^{(l+1)(t)(t)}) &l<n
		\end{cases} 
		\\
		%\delta^{(l)(t-c)(t)} &=
		%\begin{cases}
		%	f'(z^{(l)(t-c)}) \circ ((H^{(l)})^T \delta^{(l)(t-c+1)(t)}) &l=n-1 \\
		%	f'(z^{(l)(t-c)}) \circ ((H^{(l)})^T \delta^{(l)(t-c+1)(t)} + \\
		%	 (W^{(l+1)})^T \delta^{(l+1)(t-c)(t)}) &l<n-1
		%\end{cases} 
		%\\
		\gamma^{(l)(t)} &= 
		\begin{cases}
		\delta^{(l)(t)(t)} &t=T
		\\
		\delta^{(l)(t)(t)} + f'(z^{(l)(t)}) \circ ((H^{(l)})^T \gamma^{(l)(t+1)}) &l=n-1
		\\
		f'(z^{(l)(t)}) \circ ((H^{(l)})^T \gamma^{(l)(t+1)} + \\ (W^{(l+1)})^T \gamma^{(l+1)(t)}) &l<n-1
		\end{cases}
		\\
		\nabla_{H^{(l)}} J &= \frac{1}{T} \sum_{t=1}^{T} \gamma^{(l)(t)} (h^{(l)(t-1)})^T
		\\
		\nabla_{W^{(l)}} J &= 
		\begin{cases}
		\frac{1}{T} \sum_{t=1}^{T}\delta^{(n)(t)(t)} (h^{(n-1)(t)})^T &l=n\\
		\frac{1}{T} \sum_{t=1}^{T} \gamma^{(l)(t)} (h^{(l-1)(t)})^T &l<n
		\end{cases}		
		\\
		\nabla_{b^{(l)}} J &= 
		\begin{cases}
		\frac{1}{T} \sum_{t=1}^{T}\delta^{(n)(t)(t)} &l=n \\
		\frac{1}{T} \sum_{t=1}^{T} \gamma^{(l)(t)} &l<n
		\end{cases}
	\end{align}
\end{document}
